lib/Marshalling/GenericMarshalling.i.dfy
@@ -6,7 +6,6 @@ include "Seqs.i.dfy"
 include "Util.i.dfy"
 include "../Base/NativeArrays.s.dfy"
 include "../Base/PackedInts.s.dfy"
-include "../Buckets/PackedKV.i.dfy"
 
 module GenericMarshalling {
 //import opened Util__be_sequences_s
